Fix defer

new/golang/defn/defer.v
@@ -3,12 +3,14 @@ From New.golang.defn Require Import exception.
 Section defn.
 Context `{!ffi_syntax}.
 
+Definition deferType := go.FunctionType (go.Signature [] None).
+
 Definition wrap_defer : val :=
   λ: "body",
-    let: "$defer" := (GoAlloc funcT #()) in
-    "$defer" <-[go.FunctionType] #(func.mk <> <> #());;
+    let: "$defer" := GoAlloc deferType #() in
+    "$defer" <-[deferType] #(func.mk <> <> #());;
     let: "$func_ret" := exception_do ("body" "$defer") in
-    (![go.FunctionType] "$defer") #();;
+    (![deferType] "$defer") #();;
     "$func_ret".
 
 End defn.
