new/golang/defn/slice.v
@@ -1,5 +1,5 @@
 From Perennial Require Import base.
-From New.golang.defn Require Export loop assume.
+From New.golang.defn Require Export loop assume predeclared.
 
 Definition slice_index_ref `{GoContext} (elem_type : go.type) (i : Z) (s : slice.t) : loc :=
   array_index_ref elem_type i s.(slice.ptr).
@@ -17,23 +17,23 @@ Definition _new_cap : val :=
 
 Definition for_range (elem_type : go.type) : val :=
   λ: "s" "body",
-  let: "i" := GoAlloc go.int64 #() in
-  for: (λ: <>, int_lt (![go.int64] "i")
-          (FuncCall len [go.TypeLit $ go.SliceType elem_type]) "s") ;
-                      (λ: <>, "i" <-[go.int64] (![go.int64] "i") + #(W64 1)) :=
-    (λ: <>, "body" (![go.int64] "i") (![elem_type] (IndexRef (go.SliceType elem_type)) "s" (![go.int64] "i")))
+  let: "i" := GoAlloc go.int #() in
+  for: (λ: <>, int_lt (![go.int] "i")
+          (FuncCall go.len [go.TypeLit $ go.SliceType elem_type]) "s") ;
+                      (λ: <>, "i" <-[go.int] (![go.int] "i") + #(W64 1)) :=
+    (λ: <>, "body" (![go.int] "i") (![elem_type] (IndexRef (go.SliceType elem_type)) "s" (![go.int] "i")))
 .
 
 (* Takes in a list as input, and turns it into a heap-allocated slice. *)
 Definition literal (elem_type : go.type) (len : Z) : val :=
   λ: "elems",
   let st : go.type := go.SliceType elem_type in
-  let: "s" := FuncCall make2 [st] "len" in
+  let: "s" := FuncCall go.make2 [st] "len" in
   let: "l" := ref "elems" in
-  let: "i" := GoAlloc go.int64 #() in
-  (for: (λ: <>, int_lt (![go.int64] "i") "len") ; (λ: <>, "i" <-[go.int64] ![go.int64] "i" + #(W64 1)) :=
+  let: "i" := GoAlloc go.int #() in
+  (for: (λ: <>, int_lt (![go.int] "i") "len") ; (λ: <>, "i" <-[go.int] ![go.int] "i" + #(W64 1)) :=
      (λ: <>,
-        do: (IndexRef st "s" (![go.int64] "i") <-[elem_type] (Index (go.ArrayType len elem_type) "elems" "i")))) ;;
+        do: (IndexRef st "s" (![go.int] "i") <-[elem_type] (Index (go.ArrayType len elem_type) "elems" "i")))) ;;
   "s".
 
 End goose_lang.
@@ -45,7 +45,7 @@ Module go.
 Class SliceSemantics {ext : ffi_syntax} `{!GoContext} :=
 {
   make3_slice elem_type :
-    #(functions make3 [go.TypeLit $ go.SliceType elem_type]) =
+    #(functions go.make3 [go.TypeLit $ go.SliceType elem_type]) =
     (λ: "len" "cap",
        if: (int_lt "cap" "len") then Panic "makeslice: cap out of range" else #();;
        if: (int_lt "len" #(W64 0)) then Panic "makeslice: len out of range" else #();;
@@ -58,8 +58,8 @@ Class SliceSemantics {ext : ffi_syntax} `{!GoContext} :=
          InternalMakeSlice ("p", "len", "cap"))%V;
 
   make2_slice elem_type :
-    #(functions make2 [go.TypeLit $ go.SliceType elem_type]) =
-    (λ: "sz", FuncCall make3 [go.TypeLit $ go.SliceType elem_type] #() "sz" "sz")%V;
+    #(functions go.make2 [go.TypeLit $ go.SliceType elem_type]) =
+    (λ: "sz", FuncCall go.make3 [go.TypeLit $ go.SliceType elem_type] #() "sz" "sz")%V;
 
   index_ref_slice elem_type i s (Hrange : 0 ≤ i < sint.Z s.(slice.len)) :
     index_ref (go.SliceType elem_type) i #s = #(slice_index_ref elem_type i s);
@@ -68,46 +68,46 @@ Class SliceSemantics {ext : ffi_syntax} `{!GoContext} :=
     index (go.SliceType elem_type) i #s =
     GoLoad elem_type $ (Index $ go.SliceType elem_type) #(W64 i) #s;
   len_slice elem_type :
-    #(functions len [go.TypeLit $ go.SliceType elem_type]) =
+    #(functions go.len [go.TypeLit $ go.SliceType elem_type]) =
     (λ: "s", InternalLen (go.SliceType elem_type) "s")%V;
 
   cap_slice elem_type :
-    #(functions cap [go.TypeLit $ go.SliceType elem_type]) =
+    #(functions go.cap [go.TypeLit $ go.SliceType elem_type]) =
     (λ: "s", InternalCap (go.SliceType elem_type) "s")%V;
 
-  copy_underlying t : functions copy [t] = functions copy [to_underlying t];
+  copy_underlying t : functions go.copy [t] = functions go.copy [to_underlying t];
   copy_slice elem_type :
-    #(functions copy [go.TypeLit $ go.SliceType elem_type]) =
+    #(functions go.copy [go.TypeLit $ go.SliceType elem_type]) =
     (λ: "dst" "src",
        let st : go.type := go.SliceType elem_type in
-       let: "i" := GoAlloc go.int64 #() in
-       (for: (λ: <>, int_lt (![go.int64] "i") (FuncCall len [st] "dst") &&
-                (int_lt (![go.int64] "i") (FuncCall len [st] "src"))) ; (λ: <>, Skip) :=
+       let: "i" := GoAlloc go.int #() in
+       (for: (λ: <>, int_lt (![go.int] "i") (FuncCall go.len [st] "dst") &&
+                (int_lt (![go.int] "i") (FuncCall go.len [st] "src"))) ; (λ: <>, Skip) :=
           (λ: <>,
-             do: (let: "i_val" := ![go.int64] "i" in
+             do: (let: "i_val" := ![go.int] "i" in
                   IndexRef st "dst" "i_val"
                       <-[elem_type] ![elem_type] (IndexRef st "src" "i_val");;
-                  "i" <-[go.int64] "i_val" + #(W64 1))));;
-       ![go.int64] "i")%V;
+                  "i" <-[go.int] "i_val" + #(W64 1))));;
+       ![go.int] "i")%V;
 
-  append_underlying t : functions append [t] = functions append [to_underlying t];
+  append_underlying t : functions go.append [t] = functions go.append [to_underlying t];
   append_slice elem_type :
-    #(functions append [go.TypeLit $ go.SliceType elem_type]) =
+    #(functions go.append [go.TypeLit $ go.SliceType elem_type]) =
     (λ: "s" "x",
        let st : go.type := go.SliceType elem_type in
-       let: "new_len" := sum_assume_no_overflow_signed (FuncCall len [st] "s")
-                           (FuncCall len [st] "x") in
-       if: (FuncCall cap [st] "s") ≥ "new_len" then
+       let: "new_len" := sum_assume_no_overflow_signed (FuncCall go.len [st] "s")
+                           (FuncCall go.len [st] "x") in
+       if: (FuncCall go.cap [st] "s") ≥ "new_len" then
          (* "grow" s to include its capacity *)
          let: "s_new" := Slice st "s" #(W64 0) "new_len" in
          (* copy "x" past the original "s" *)
-         FuncCall copy [st] (Slice st "s_new" (FuncCall len [st] "s") "new_len") "x";;
+         FuncCall go.copy [st] (Slice st "s_new" (FuncCall go.len [st] "s") "new_len") "x";;
          "s_new"
        else
          let: "new_cap" := slice._new_cap "new_len" in
-         let: "s_new" := FuncCall make3 [st] "new_len" "new_cap" in
-         FuncCall copy [st] "s_new" "s" ;;
-         FuncCall copy [st] (Slice st "s_new" (FuncCall len [st] "s") "new_len") "x" ;;
+         let: "s_new" := FuncCall go.make3 [st] "new_len" "new_cap" in
+         FuncCall go.copy [st] "s_new" "s" ;;
+         FuncCall go.copy [st] (Slice st "s_new" (FuncCall go.len [st] "s") "new_len") "x" ;;
          "s_new")%V;
 
   array_index_ref_0 t l : array_index_ref t 0 l = l;
