new/golang/theory/defer.v
@@ -1,22 +1,23 @@
-From New.golang.theory Require Import exception mem.
+From New.golang.theory Require Import exception mem postlifting.
 From New.golang.defn Require Import defer.
 
 Section proof.
-  Context `{ffi_sem: ffi_semantics} `{!ffi_interp ffi} `{!heapGS Σ}.
+Context `{ffi_sem: ffi_semantics} `{!ffi_interp ffi} `{!heapGS Σ}
+          {Hcore : go.CoreSemantics}.
 
-  Lemma wp_with_defer e Φ :
-    (∀ (defer : loc),
-       defer ↦ (func.mk <> <> #())%V -∗
-       WP (let: "$func_ret" := exception_do (subst "$defer" #defer e) in ![funcT] #defer #();; "$func_ret")
-         {{ Φ }}) -∗
-    WP (wrap_defer #(func.mk <> ("$defer" : string) e)) {{ Φ }}.
-  Proof.
-    iIntros "Hwp".
-    wp_call.
-    wp_alloc defer as "defer". wp_pures.
-    wp_bind.
-    wp_apply (wp_mem_store with "defer"). iIntros "?".
-    wp_pures. iApply "Hwp". iFrame.
-  Qed.
+Lemma wp_with_defer e Φ :
+  (∀ (defer : loc),
+     defer ↦ (func.mk <> <> #())%V -∗
+     WP (let: "$func_ret" := exception_do (subst "$defer" #defer e) in ![deferType] #defer #();; "$func_ret")
+       {{ Φ }}) -∗
+  WP (wrap_defer #(func.mk <> ("$defer" : string) e)) {{ Φ }}.
+Proof.
+  iIntros "Hwp".
+  wp_call.
+  wp_alloc defer as "defer". wp_pures.
+  wp_bind.
+  wp_apply (wp_store with "defer"). iIntros "?".
+  wp_pures. iApply "Hwp". iFrame.
+Qed.
 
 End proof.
